src/base_logic/lib/mono_nat.v
@@ -16,4 +16,12 @@ Global Instance mono_nat_lb_own_discretizable (γ: gname) n :
   Discretizable (mono_nat_lb_own γ n).
 Proof. rewrite mono_nat.mono_nat_lb_own_unseal. apply _. Qed.
 
+(* TODO UPSTREAM https://gitlab.mpi-sws.org/iris/iris/-/merge_requests/817 *)
+Lemma mono_nat_lb_own_0 γ :
+  ⊢ |==> mono_nat_lb_own γ 0.
+Proof.
+  rewrite mono_nat.mono_nat_lb_own_unseal /mono_nat.mono_nat_lb_own_def.
+  iApply (own_unit mono_nat.mono_natUR).
+Qed.
+
 End iris.
