src/program_proof/mvcc/examples_proof.v
@@ -1,5 +1,5 @@
 (* Import definitions/theorems of the Perennial framework with the disk FFI. *)
-From Perennial.program_proof Require Export disk_prelude.
+From Perennial.program_proof Require Export grove_prelude.
 (* Import Coq model of our Goose program. *)
 From Goose.github_com.mit_pdos.go_mvcc Require Import examples.
 From Perennial.program_proof.mvcc Require Import mvcc_ghost txn_proof.
